fixed def of genproof_spec; implemented genproof

Structures/Types.v
@@ -60,15 +60,120 @@ Qed.
 
 Parameter genproof : list Certificate -> list Address.
 
-Axiom genproof_spec : 
+Definition genproof_can_detect (genproof : list Certificate -> list Address) : Prop :=
   forall certs n, In n (genproof certs) <-> 
-    exists v1 v2 nsigs1 nsigs2,
+    exists v1 v2 sig1 sig2 nsigs1 nsigs2,
       v1 <> v2 /\
       In (v1, nsigs1) certs /\
       In (v2, nsigs2) certs /\
-      In (n, sign v1 (key_map n)) nsigs1 /\
-      In (n, sign v2 (key_map n)) nsigs2.
+      In (n, sig1) nsigs1 /\
+      In (n, sig2) nsigs2.
 
-Axiom genproof_nodup : forall certs, NoDup (genproof certs).
+Record genproof_spec (genproof : list Certificate -> list Address) : Prop := {
+  _ : genproof_can_detect genproof;
+  _ : forall certs, NoDup (genproof certs)
+}.
+
+Axiom genproof_correct : genproof_spec genproof.
+
+(* should give a concrete genproof which does not depend on knowing
+    key_map so that it is not vacuous
+  TODO for now simply keep it here
+*)
+
+Definition genproof_simple_aux_aux (c : Certificate) (certs : list Certificate) :=
+  (List.flat_map 
+    (fun c' => if Value_eqdec (fst c) (fst c') 
+                then nil 
+                else (filter 
+                  (fun n => In_dec Address_eqdec n (map fst (snd c))) 
+                  (map fst (snd c')))) certs).
+
+Fixpoint genproof_simple_aux (certs : list Certificate) : list Address :=
+  match certs with
+  | nil => nil
+  | c :: certs' => (genproof_simple_aux_aux c certs') ++ (genproof_simple_aux certs')
+  end.
+
+Definition genproof_simple (certs : list Certificate) : list Address :=
+  nodup Address_eqdec (genproof_simple_aux certs).
+
+Lemma genproof_simple_aux_aux_can_detect v nsigs certs n : 
+  In n (genproof_simple_aux_aux (v, nsigs) certs) <-> 
+  exists v' nsigs',
+    v <> v' /\
+    In (v', nsigs') certs /\
+    In n (map fst nsigs) /\
+    In n (map fst nsigs').
+Proof.
+  induction certs as [ | (v_, nsigs_) certs IH ].
+  - firstorder.
+  - simpl.
+    rewrite -> in_app_iff, -> IH.
+    clear IH.
+    destruct (Value_eqdec v v_) as [ <- | Hvneq ].
+    + firstorder.
+      congruence.
+    + rewrite -> filter_In.
+      (* awkward ... *)
+      assert (in_dec Address_eqdec n (map fst nsigs) <-> In n (map fst nsigs)) as Hp.
+      {
+        unfold is_true.
+        now destruct (in_dec Address_eqdec n (map fst nsigs)).
+      }
+      rewrite -> Hp.
+      intuition firstorder congruence.
+Qed.
+
+Lemma genproof_simple_aux_can_detect certs n : In n (genproof_simple_aux certs) <-> 
+  exists v1 v2 nsigs1 nsigs2,
+    v1 <> v2 /\
+    In (v1, nsigs1) certs /\
+    In (v2, nsigs2) certs /\
+    In n (map fst nsigs1) /\
+    In n (map fst nsigs2).
+Proof.
+  induction certs as [ | (v, nsigs) certs IH ].
+  - firstorder.
+  - simpl.
+    rewrite -> in_app_iff, -> IH, -> genproof_simple_aux_aux_can_detect.
+    clear IH.
+    split.
+    + intros [ (v' & nsigs' & Hvneq & Hin' & Hin_nsigs & Hin_nsigs') | 
+        (v1 & v2 & nsigs1 & nsigs2 & Hvneq & Hin1 & Hin2 & Hin_nsigs1 & Hin_nsigs2) ].
+      * exists v, v', nsigs, nsigs'.
+        intuition.
+      * exists v1, v2, nsigs1, nsigs2.
+        intuition.
+    + intros (v1 & v2 & nsigs1 & nsigs2 & Hvneq & [ Hin1 | Hin1 ] & [ Hin2 | Hin2 ] & Hin_nsigs1 & Hin_nsigs2).
+      all: try congruence.
+      1-2: left.
+      1: exists v2, nsigs2.
+      2: exists v1, nsigs1.
+      1-2: intuition congruence.
+      right.
+      exists v1, v2, nsigs1, nsigs2.
+      intuition.
+Qed.
+
+Lemma genproof_simple_correct : genproof_spec genproof_simple.
+Proof.
+  unfold genproof_simple.
+  constructor.
+  - hnf.
+    intros.
+    rewrite -> nodup_In, -> genproof_simple_aux_can_detect.
+    repeat setoid_rewrite -> in_map_iff.
+    split.
+    + intros (v1 & v2 & nsigs1 & nsigs2 & ? & ? & ? & ((n', sig1) & Htmp1 & ?) & ((n'', sig2) & Htmp2 & ?)).
+      simpl in Htmp1, Htmp2.
+      subst n' n''.
+      now exists v1, v2, sig1, sig2, nsigs1, nsigs2.
+    + intros (v1 & v2 & sig1 & sig2 & nsigs1 & nsigs2 & ? & ? & ? & ? & ?).
+      exists v1, v2, nsigs1, nsigs2.
+      firstorder.
+  - intros. 
+    now apply NoDup_nodup.
+Qed.
 
 End Types.
